Correction

core_c/operations_term.v
@@ -9,7 +9,6 @@ Local Coercion Z.of_nat: nat >-> Z.
 
 Section operations_definitions2.
   Context `{Env K}.
-
   (* ACSL values *)
   Inductive val_term (K : iType) : iType :=
   | ValC : val K -> val_term K
@@ -62,6 +61,7 @@ Section operations_definitions2.
     | ValC v,_ => ValC(val_unop (tun_to_un op) v)
     | _,_ => v
     end.
+
   
   (* New arithop function which takes the divZ constructor when there is a division by zero *)
   Definition new_arithop (op : arithop)(x y : Z) (τi1 τi2 : int_type K) : Z  :=
@@ -71,34 +71,17 @@ Section operations_definitions2.
     end.
 
   (* New operation on int which take divide by zero in account *)
-  Definition new_int_binop (op : binop) (x1 x2 : Z) (τi1 τi2 : int_type K) : Z :=
-    match op with
-    | ArithOp op => new_arithop op x1 x2 τi1 τi2
-    | _ => int_binop op x1 τi1 x2 τi2
-    end.
+  Definition new_int_binop (op : arithop) (x1 x2 : Z) (τi1 τi2 : int_type K) : Z :=
+     new_arithop op x1 x2 τi1 τi2
+    .
   
   (* New operation on base_val which take divide by zero in account *)
   Definition new_base_val_binop (en : env K) (op : binop) (v1 v2 : base_val K): base_val K :=
-    match v1, v2 with
-    | VInt τi1 x1, VInt τi2 x2 => VInt (int_binop_type_of op τi1 τi2) (new_int_binop op x1 x2 τi1 τi2)
-    |_,_ => base_val_binop en op v1 v2
+    match v1, v2, op with
+    | VInt τi1 x1, VInt τi2 x2, ArithOp aop =>
+        VInt (int_binop_type_of op τi1 τi2) (new_int_binop aop x1 x2 τi1 τi2)
+    |_,_, _ => base_val_binop en op v1 v2
     end.
-  
-  (* Predicate to know when a comparison operation is allowed *)
-  Definition valt_compop_ok (en : env K) (v1 v2 : val_term K) : Prop :=
-    match v1,v2 with
-    | VInteger _, VInteger _ => True
-    | VInteger _, ValC( VBase (VInt _ _)) => True
-    | ValC( VBase (VInt _ _)), VInteger _ => True
-    | ValC(VBase (VPtr _)), ValC (VBase (VPtr _)) => True
-    | ValC(VStruct _ _), ValC(VStruct _ _)=> True
-    | ValC(VUnion _ _ _), ValC( VUnion _ _ _)=> True
-    | ValC(VUnionAll _ _), ValC(VUnionAll _ _) => True
-    | ValC(VUnionAll _ _), ValC( VUnion _ _ _) => True
-    | ValC( VUnion _ _ _) , ValC(VUnionAll _ _) => True
-    | _, _ => False
-    end.
-
 
   (* New operation on c values which take divide by zero in account *)
   Definition new_val_binop (en : env K) (op : binop) (v1 v2 : val K) : val K :=
@@ -106,7 +89,7 @@ Section operations_definitions2.
     | VBase vb1, VBase vb2 => VBase (new_base_val_binop en op vb1 vb2)
     | _,_ => val_binop en op v1 v2
     end.
-
+  
   (*Last operation to sumup all modifications : arithmetic between C int and acsl integer 
     (convert
     to acsl integer) *)
@@ -116,8 +99,12 @@ Section operations_definitions2.
     | VInteger n1, ValC (VBase (VInt t n2)), TArithOp aop => VInteger (arithopZ aop n1 n2)
     | ValC (VBase (VInt t n1)), VInteger n2, TArithOp aop => VInteger (arithopZ aop n1 n2)
     | ValC v1, ValC v2, _ => ValC (new_val_binop en (tbin_to_bin op) v1 v2)
+    | VInteger n1, ValC(ptrV p), TArithOp aop => ValC (ptrV (ptr_plus en n1 p))
+    | ValC(ptrV p), VInteger n1, TArithOp aop => ValC (ptrV (ptr_plus en n1 p))
     | _,_,_ => vt1
     end.
+
+
 
   (* Inductive predicate used to know if a value and a list of values can be compared (predicate used in proofs) *)
   Inductive comparable : val K -> Prop :=
@@ -130,73 +117,75 @@ Section operations_definitions2.
   | cmp_nil : comparable_list []
   | cmp_cons : forall v l, comparable v -> comparable_list l -> comparable_list (v::l).
 
+   
    (* Equality between C values *)
-  Inductive eq_val : env K -> val K -> val K -> Prop :=
-  | eq_base : forall(en : env K) (vb1 vb2 : base_val K),
+  Inductive eq_val : env K -> val K -> val K -> mem K -> Prop :=
+  | eq_base : forall(en : env K) (vb1 vb2 : base_val K)(m : mem K),
+      base_val_binop_ok en m (CompOp EqOp) vb1 vb2 ->
       new_base_val_binop en (CompOp EqOp) vb1 vb2 = VInt sintT 1 ->
-      eq_val en (VBase vb1) (VBase vb2)
+      eq_val en (VBase vb1) (VBase vb2) m
   | eq_struct : forall (en : env K)
-                      (lval1 lval2 : list (val K)) (tag1 tag2 : tag),
-      eq_list  en lval1 lval2 
-      -> eq_val en (VStruct tag1 lval1) (VStruct tag2 lval2)
-  | eq_union1 : forall (en : env K)(v1 v2 vu1 vu2 : val K)(tag1 tag2 : tag)(n1 n2 : nat),
+                      (lval1 lval2 : list (val K)) (tag1 tag2 : tag)(m : mem K),
+      eq_list  en lval1 lval2 m
+      -> eq_val en (VStruct tag1 lval1) (VStruct tag2 lval2) m
+  | eq_union1 : forall (en : env K)(v1 v2 vu1 vu2 : val K)(tag1 tag2 : tag)(n1 n2 : nat)(m : mem K),
       v1 = VUnion tag1 n1 vu1 ->
       v2 = VUnion tag2 n2 vu2  ->
       val_flatten en v1 = val_flatten en v2 ->
-      eq_val en v1 v2
+      eq_val en v1 v2 m
   | eq_union2 : forall (en : env K) (v1 v2 vu1 : val K)
-                       (tag1 tag2 : tag)(n1 : nat) (lval2 : list (val K)),
+                       (tag1 tag2 : tag)(n1 : nat) (lval2 : list (val K))(m : mem K),
       v1 = VUnion tag1 n1 vu1 ->
       v2 = VUnionAll tag2 lval2 ->
       val_flatten en v1 = val_flatten en v2 ->
-      eq_val en v1 v2
+      eq_val en v1 v2 m
   | eq_union3 : forall (en : env K) (v1 v2 vu2 : val K)
-                       (tag1 tag2 : tag)(n2 : nat) (lval1 : list (val K)),
+                       (tag1 tag2 : tag)(n2 : nat) (lval1 : list (val K))(m : mem K),
       v2 = VUnion tag2 n2 vu2 ->
       v1 = VUnionAll tag1 lval1 ->
       val_flatten en v1 = val_flatten en v2 ->
-      eq_val en v1 v2
+      eq_val en v1 v2 m
   | eq_union4 : forall (en : env K) (v1 v2 : val K)
-                       (tag1 tag2 : tag) (lval1 lval2 : list (val K)),
+                       (tag1 tag2 : tag) (lval1 lval2 : list (val K))( m : mem K),
       v2 = VUnionAll tag2 lval2 ->
       v1 = VUnionAll tag1 lval1 ->
       val_flatten en v1 = val_flatten en v2 ->
-      eq_val en v1 v2
-  | eq_same : forall (en : env K)(v1 v2 : val K),
+      eq_val en v1 v2 m
+  | eq_same : forall (en : env K)(v1 v2 : val K)(m : mem K),
       v1 = v2 ->
-      eq_val en v1 v2
+      eq_val en v1 v2 m
              
   (* Equality between list of C values *)
-  with eq_list : env K -> list (val K) -> list (val K) -> Prop :=
-  | eq_list_empty : forall (en : env K) ,
-      eq_list  en [] []
-  | eq_list_cons : forall (en : env K) (v1 v2 : val K) (lvq1 lvq2: list (val K)),
-      eq_val en v1 v2 ->
-      eq_list en lvq1 lvq2 ->
-      eq_list en (v1::lvq1) (v2::lvq2)
-  | eq_list_same : forall (en : env K) (l : list (val K)),
-      eq_list en l l.
+  with eq_list : env K -> list (val K) -> list (val K) -> mem K -> Prop :=
+  | eq_list_empty : forall (en : env K) (m : mem K) ,
+      eq_list  en [] [] m
+  | eq_list_cons : forall (en : env K) (v1 v2 : val K) (lvq1 lvq2: list (val K))(m : mem K),
+      eq_val en v1 v2 m ->
+      eq_list en lvq1 lvq2 m ->
+      eq_list en (v1::lvq1) (v2::lvq2) m
+  | eq_list_same : forall (en : env K) (l : list (val K))(m : mem K),
+      eq_list en l l m.
   
   (* Comparison of values *)
   Inductive comp_val : compop -> env K -> val K -> val K -> Prop :=
-  | eq_value : forall (en : env K)(v1 v2 : val K),
-      eq_val en v1 v2 -> comp_val EqOp en v1 v2
+  | eq_value : forall (en : env K)(v1 v2 : val K)(m : mem K),
+      eq_val en v1 v2 m  -> comp_val EqOp en v1 v2
   | comp_other : forall (op : compop)(en : env K) (v1 v2 : val K),
       new_val_binop en (CompOp op) v1 v2 = VBase (VInt sintT 1) ->
       comp_val op en v1 v2.
 
   (* Equality between ACSL values *)
-  Inductive eq_valt : env K -> val_term K -> val_term K -> Prop :=
-  | eq_valc : forall (en : env K)(v1 v2 : val K),
-      eq_val en v1 v2 -> eq_valt en (ValC v1) (ValC v2)
-  | eq_integer : forall (en : env K) (x y : Z),
-      x = y -> eq_valt en (VInteger x) (VInteger y)
-  | eq_integerInt : forall (en : env K) (x y : Z) (t : int_type K),
-      x = y -> eq_valt en (VInteger x) (ValC (VBase (VInt t y)))
-  | eq_intInteger : forall (en : env K) (x y : Z) (t : int_type K),
-      x = y -> eq_valt en (ValC (VBase (VInt t x))) (VInteger y)
-  | eq_samet : forall (en : env K) (v : val_term K),
-      eq_valt en v v.
+  Inductive eq_valt : env K -> val_term K -> val_term K -> mem K-> Prop :=
+  | eq_valc : forall (en : env K)(v1 v2 : val K)(m : mem K),
+      eq_val en v1 v2 m -> eq_valt en (ValC v1) (ValC v2) m
+  | eq_integer : forall (en : env K) (x y : Z)(m : mem K),
+      x = y -> eq_valt en (VInteger x) (VInteger y) m
+  | eq_integerInt : forall (en : env K) (x y : Z) (t : int_type K)(m : mem K),
+      x = y -> eq_valt en (VInteger x) (ValC (VBase (VInt t y))) m
+  | eq_intInteger : forall (en : env K) (x y : Z) (t : int_type K)(m : mem K),
+      x = y -> eq_valt en (ValC (VBase (VInt t x))) (VInteger y) m
+  | eq_samet : forall (en : env K) (v : val_term K)(m : mem K),
+      eq_valt en v v m.
       
   (* Comparison of integers *)
   Inductive comp_int : compop -> Z -> Z -> Prop :=
@@ -208,8 +197,8 @@ Section operations_definitions2.
   Inductive comp_valt : compop -> env K -> val_term K -> val_term K -> Prop :=
   | comp_valc : forall (en : env K)(v1 v2 : val K)(op : compop),
       comp_val op en v1 v2 -> comp_valt op en (ValC v1) (ValC v2)
-  | eq_valuet : forall (en : env K)(v1 v2 : val_term K),
-      eq_valt en v1 v2 -> comp_valt EqOp en v1 v2
+  | eq_valuet : forall (en : env K)(v1 v2 : val_term K)(m : mem K),
+      eq_valt en v1 v2 m -> comp_valt EqOp en v1 v2
   | comp_valInt : forall (en : env K)(x y : Z)(op : compop),
       comp_int op x y -> comp_valt op en (VInteger x) (VInteger y)
   | comp_intInteger : forall (en : env K)(x y : Z)(op : compop)(ty : int_type K),
@@ -233,22 +222,76 @@ Section operations_definitions2.
     constructor.
     reflexivity.
   Qed.
-
+  
   (* Assume that equality furnished in CH2O is symmetric*)
-  Axiom eq_val_sym : forall(v1 v2 : base_val K)(en : env K),
+  Axiom eq_bval_sym : forall(v1 v2 : base_val K)(en : env K)(m : mem K),
+      base_val_binop_ok en m (CompOp EqOp) v1 v2 ->
+      base_val_binop en (CompOp EqOp) v1 v2 = (intV{sintT} 1)%B ->
+      base_val_binop en (CompOp EqOp) v2 v1 = (intV{sintT} 1)%B.
+  
+
+  (* Proof that equality in CH2O with our modification is symetric *)
+  Lemma eq_val_sym : forall(v1 v2 : base_val K)(en : env K)(m : mem K),
+      base_val_binop_ok en m (CompOp EqOp) v1 v2 ->
       new_base_val_binop en (CompOp EqOp) v1 v2 = (intV{sintT} 1)%B ->
       new_base_val_binop en (CompOp EqOp) v2 v1 = (intV{sintT} 1)%B.
-   
-  (* Assume that equality furnished in CH2O is reflexive*)
-  Axiom eq_val_refl : forall(v : base_val K)(en : env K),
-      new_base_val_binop en (CompOp EqOp) v v = (intV{sintT} 1)%B.
-  
+    Proof.
+      intros.
+      destruct v1, v2.
+      all : try unfold base_val_binop_ok in H0. all : try contradiction.
+      unfold new_base_val_binop.
+      unfold new_base_val_binop in H1.
+      apply (eq_bval_sym (intV{i} z) (intV{i0} z0) en m).
+      unfold base_val_binop_ok. assumption.
+      assumption.
+      unfold new_base_val_binop.
+      unfold new_base_val_binop in H1.
+      apply (eq_bval_sym (ptrV p) (ptrV p0) en m). unfold base_val_binop_ok.
+      assumption. assumption.
+    Qed.
+
+
+    
   (* Assume that equality furnished in CH2O is transitive *)
-  Axiom eq_val_trans : forall (v1 v2 v3 : base_val K)(en : env K),
+    Axiom eq_bval_trans : forall (v1 v2 v3 : base_val K)(en : env K)(m : mem K),
+      base_val_binop_ok en m (CompOp EqOp) v1 v2 ->
+      base_val_binop_ok en m (CompOp EqOp) v2 v3 ->
+      base_val_binop en (CompOp EqOp) v1 v2 = (intV{sintT} 1)%B ->
+      base_val_binop en (CompOp EqOp) v2 v3 = (intV{sintT} 1)%B ->
+      base_val_binop en (CompOp EqOp) v1 v3 = (intV{sintT} 1)%B.
+   
+  (* Proof that equality in CH2O with our modification is transitive *)
+    Lemma eq_val_trans : forall (v1 v2 v3 : base_val K)(en : env K)(m : mem K),
+      base_val_binop_ok en m (CompOp EqOp) v1 v2 ->
+      base_val_binop_ok en m (CompOp EqOp) v2 v3 ->
       new_base_val_binop en (CompOp EqOp) v1 v2 = (intV{sintT} 1)%B ->
       new_base_val_binop en (CompOp EqOp) v2 v3 = (intV{sintT} 1)%B ->
       new_base_val_binop en (CompOp EqOp) v1 v3 = (intV{sintT} 1)%B.
 
+    Proof.
+      intros.
+      destruct v1, v2, v3.
+      all : try unfold base_val_binop_ok in H0, H1. all : try contradiction.
+      unfold new_base_val_binop in H2, H3.
+      unfold new_base_val_binop.
+      apply (eq_bval_trans (intV{i} z) (intV{i0} z0) (intV{i1} z1) en m).
+      all : try unfold base_val_binop_ok. all : try assumption.
+      unfold new_base_val_binop in H2, H3.
+      unfold new_base_val_binop.
+      apply (eq_bval_trans (ptrV p) (ptrV p0) (ptrV p1) en m).
+      all : try unfold base_val_binop_ok.
+      all : try assumption.
+    Qed.
+
+    (*Assume that the comparison condition is symetric*)
+    Axiom eq_base_val_ok_sym : forall en m vb1 vb2,
+      base_val_binop_ok en m (CompOp EqOp) vb1 vb2 -> base_val_binop_ok en m (CompOp EqOp) vb2 vb1.
+    (*Assume that the comparison condtion is transitive*)
+  Axiom eq_base_val_ok_trans : forall en m vb1 vb2 vb3,
+      base_val_binop_ok en m (CompOp EqOp) vb1 vb2 ->
+      base_val_binop_ok en m (CompOp EqOp) vb2 vb3 ->
+      base_val_binop_ok en m (CompOp EqOp) vb1 vb3.
+      
   (* Assume that comparing two C int is equivalent to compare their int part in their 
 abstract representation*)
   Axiom int_cast_eq : forall (t t2 : int_type K) (en : env K) (x y : Z),
@@ -294,27 +337,31 @@ abstract representation*)
                                     end in val_list_ind l
       end.
   End val_ind.
+ 
   
+  Scheme eq_val_rec := Induction for eq_val Sort Prop
+      with eq_list_rec := Induction for eq_list Sort Prop.
+
+   
   (* Proof of reflexivity of the equality between ACSL values *)
-  Lemma eq_valt_reflexive v en : eq_valt en v v.
+  Lemma eq_valt_reflexive v en m : eq_valt en v v m.
   Proof.
     intros.
     apply eq_samet.
   Qed.
   
-  Scheme eq_val_rec := Induction for eq_val Sort Prop
-      with eq_list_rec := Induction for eq_list Sort Prop.
-
-
   (* Proof of symetry of the equality between C values *)
-  Lemma eq_val_symetric : forall(v1 v2 : val K)(en : env K),
-      eq_val en v1 v2 -> eq_val en v2 v1.
+Lemma eq_val_symetric : forall(v1 v2 : val K)(en : env K)(m : mem K),
+    eq_val en v1 v2 m -> eq_val en v2 v1 m.
   Proof.
-    intros vl vr en.
+    intros vl vr en m Hp.
     apply (eq_val_rec
-             (λ en vl vr (_:eq_val en vl vr), eq_val en vr vl)
-             (λ en ll lr (_: eq_list en ll lr), eq_list en lr ll)).
-    - intros. apply (eq_base en0 vb2 vb1). apply (eq_val_sym vb1 vb2 en0).
+             (λ en vl vr m (_:eq_val en vl vr m), eq_val en vr vl m)
+             (λ en ll lr m (_: eq_list en ll lr m ), eq_list en lr ll m)).
+    - intros. apply (eq_base en0 vb2 vb1). apply eq_base_val_ok_sym.
+      assumption.
+      apply (eq_val_sym vb1 vb2 en0 m0).
+      assumption.
       assumption.
     - intros.  apply (eq_struct en0 lval2 lval1 tag2 tag1). assumption.
     - intros. apply (eq_union1 en0 v2 v1 vu2 vu1 tag2 tag1 n2 n1).
@@ -330,13 +377,15 @@ abstract representation*)
     - intros. apply (eq_list_cons).
       assumption. assumption.
     - intros. apply eq_list_same.
+    - intros. assumption.
   Qed.
 
+  
   (* Proof of symetry between ACSL values *) 
-  Lemma eq_val_term_symetric : forall(v1 v2 : val_term K)(en : env K),
-      eq_valt en v1 v2 -> eq_valt en v2 v1.
+  Lemma eq_val_term_symetric : forall(v1 v2 : val_term K)(en : env K)(m : mem K),
+      eq_valt en v1 v2 m -> eq_valt en v2 v1 m.
     intros. inversion H0.
-    apply eq_valc.
+    apply (eq_valc en v3 v0 m).
     apply eq_val_symetric.
     assumption.
     apply eq_integer.
@@ -347,26 +396,28 @@ abstract representation*)
     apply eq_samet.
   Qed.
 
+
+
   (* Proof of transitivity of equality between C values*)
-  Lemma eq_val_transitive : forall (v1 v2 v3 : val K) (en : env K),
-      eq_val en v1 v2 -> eq_val en v2 v3 -> eq_val en v1 v3. 
+  Lemma eq_val_transitive : forall (v1 v2 v3 : val K) (en : env K)(m : mem K),
+      eq_val en v1 v2 m -> eq_val en v2 v3 m -> eq_val en v1 v3 m.
   Proof.
-    intros v1 v2 v3 en H12.
-    
+    intros v1 v2 v3 en m H12.
     apply (eq_val_rec
-             (λ en v1 v2 (_ : eq_val en v1 v2), ∀ v3, eq_val en v2 v3 → eq_val en v1 v3)
-             (λ en l1 l2 (_ : eq_list en l1 l2), ∀ l3, eq_list en l2 l3 → eq_list en l1 l3)).
-    - intros en0 vb1 vb2 Hvb12 v3' H23. inversion H23. constructor.
-      apply (eq_val_trans vb1 vb2 vb3 en0). assumption. assumption.
+             (λ en v1 v2 m (_ : eq_val en v1 v2 m), ∀ v3, eq_val en v2 v3 m → eq_val en v1 v3 m)
+             (λ en l1 l2 m (_ : eq_list en l1 l2 m), ∀ l3, eq_list en l2 l3 m → eq_list en l1 l3 m)).
+    - intros en0 vb1 vb2 m2 Hok Hvb12 v3' H23. inversion H23. constructor.
+      apply (eq_base_val_ok_trans en0 m2 vb1 vb2 vb3). assumption. assumption.
+      apply (eq_val_trans vb1 vb2 vb3 en0 m2). assumption. assumption. assumption. assumption.
       discriminate. discriminate. discriminate. discriminate.  rewrite <- H0.
-      apply eq_base. assumption.
-    - intros en0 lval1 lval2 tag1 tag2 Hl12 IHl v3' H23. inversion H23.
+      apply eq_base. assumption. assumption.
+    - intros en0 lval1 lval2 tag1 tag2 m2 Hl12 IHl v3' H23. inversion H23.
       constructor. apply IHl. assumption. discriminate. discriminate. discriminate. discriminate.
       rewrite <- H0. 
       apply eq_struct. assumption.
-    - intros en0 v1' v2' vu1 vu2 tag1 tag2 n1 n2 H1 H2 H12' v3' H23.
+    - intros en0 v1' v2' vu1 vu2 tag1 tag2 n1 n2 m2 H1 H2 H12' v3' H23.
       inversion H23.
-      rewrite -> H2 in H4. discriminate. rewrite -> H2 in H4. discriminate.
+      rewrite -> H2 in H5. discriminate. rewrite -> H2 in H4. discriminate.
       apply (eq_union1 en0 v1' v3' vu1 vu3 tag1 tag3 n1 n3).
       assumption. assumption. rewrite -> H4 in H12'. assumption.
       apply (eq_union2 en0 v1' v3' vu1 tag1 tag3 n1 lval2). assumption. assumption.
@@ -375,8 +426,8 @@ abstract representation*)
       rewrite -> H2 in H3. discriminate.
       rewrite <- H0. apply (eq_union1 en0 v1' v2' vu1 vu2 tag1 tag2 n1 n2).
       assumption. assumption. assumption.
-    - intros en0 v1' v2' vu1 tag1 tag2 n1 lval2 H1 H2 H12' v3' H23. inversion H23. 
-      rewrite <- H4 in H2. discriminate.
+    - intros en0 v1' v2' vu1 tag1 tag2 n1 lval2 m2 H1 H2 H12' v3' H23. inversion H23. 
+      rewrite <- H5 in H2. discriminate.
       rewrite <- H4 in H2. discriminate.
       rewrite -> H0 in H2. discriminate.
       rewrite -> H0 in H2. discriminate.
@@ -386,8 +437,8 @@ abstract representation*)
       rewrite <- H12' in H4. assumption.
       rewrite <- H0. apply (eq_union2 en0 v1' v2' vu1 tag1 tag2 n1 lval2).
       assumption. assumption. assumption.
-    - intros en0 v1' v2' vu2 tag1 tag2 n2 lval1 H2 H1 H12' v3' H23. inversion H23.
-      rewrite <- H4 in H2. discriminate.
+    - intros en0 v1' v2' vu2 tag1 tag2 n2 lval1 m2 H2 H1 H12' v3' H23. inversion H23.
+      rewrite <- H5 in H2. discriminate.
       rewrite <- H4 in H2. discriminate.
       apply (eq_union3 en0 v1' v3' vu0 tag1 tag3 n0 lval1).
       assumption. assumption. rewrite <- H12' in H4. assumption.
@@ -397,8 +448,8 @@ abstract representation*)
       rewrite -> H2 in H3. discriminate.
       rewrite <- H0. apply (eq_union3 en0 v1' v2' vu2 tag1 tag2 n2 lval1 ).
       assumption. assumption. assumption.
-    - intros en0 v1' v2' tag1 tag2 lval1 lval2 H2 H1 H12' v3' H23. inversion H23.
-      rewrite <- H4 in H2. discriminate.
+    - intros en0 v1' v2' tag1 tag2 lval1 lval2 m2 H2 H1 H12' v3' H23. inversion H23.
+      rewrite <- H5 in H2. discriminate.
       rewrite <- H4 in H2. discriminate.
       rewrite -> H0 in H2. discriminate.
       rewrite -> H0 in H2. discriminate.
@@ -408,8 +459,8 @@ abstract representation*)
       assumption. assumption. rewrite <- H12' in H4. assumption.
       rewrite <- H0. apply (eq_union4 en0 v1' v2' tag1 tag2 lval1 lval2).
       assumption. assumption. assumption.
-    - intros. inversion H0. rewrite e. rewrite <- H3.
-      apply eq_base. assumption. rewrite e. rewrite <- H3.
+    - intros. inversion H0. rewrite e. rewrite <- H4.
+      apply eq_base. assumption. assumption. rewrite e. rewrite <- H3.
       apply eq_struct. assumption.
       rewrite e. apply (eq_union1 en0 v4 v5 vu1 vu2 tag1 tag2 n1 n2).
       assumption. assumption. assumption.
@@ -421,7 +472,7 @@ abstract representation*)
       assumption. assumption. assumption.
       rewrite <- H1. rewrite e. apply eq_same. reflexivity.
     - intros. inversion H0. constructor. constructor.
-    - intros en0 v0 v4 lv1 lv2 H04 IH Hl12 IHl l3 Hv41213.
+    - intros en0 v0 v4 lv1 lv2 m2 H04 IH Hl12 IHl l3 Hv41213.
       inversion Hv41213. constructor.
       apply IH. assumption.
       apply IHl. assumption.
@@ -432,116 +483,90 @@ abstract representation*)
 
   
   (* Proof of transitivity of equality between ACSL values*)
-  Lemma eq_valt_transitive : forall (v1 v2 v3 : val_term K) (en : env K),
-      valt_compop_ok en v1 v2 -> valt_compop_ok en v2 v3 -> eq_valt en v1 v2 -> eq_valt en v2 v3 -> eq_valt en v1 v3. 
-    intros v1 v2 v3 en H0 H00 H1 H2.
+  Lemma eq_valt_transitive : forall (v1 v2 v3 : val_term K) (en : env K)(m : mem K),
+      eq_valt en v1 v2 m -> eq_valt en v2 v3 m -> eq_valt en v1 v3 m. 
+    intros v1 v2 v3 en m H1 H2.
     inversion H1.
     inversion H2.
-    + apply eq_valc.
-      rewrite <- H6 in H9.
+    
+    + apply (eq_valc en v0 v6 m).
+      rewrite <- H5 in H9.
       injection H9.
       intro.
-      rewrite <- H11 in H3.
+      rewrite <- H12 in H0.
       apply (eq_val_transitive v0 v5 v6).
       assumption.
       assumption.
-    + rewrite <- H9 in H6. discriminate.
-    + rewrite <- H9 in H6. discriminate.
-    + rewrite <- H9 in H6. injection H6. intro.
-      destruct H3.
-      destruct vb1.
-      unfold new_base_val_binop in H3. unfold base_val_binop in H3.
+      
+    + rewrite <- H9 in H5. discriminate.
+    + rewrite <- H9 in H5. discriminate.
+      
+    + rewrite <- H9 in H5. injection H5. intro.
+      destruct H0.
+      destruct vb1. discriminate.
       discriminate.
-      unfold new_base_val_binop in H3. unfold base_val_binop in H3.
-      discriminate.
-      injection H11. intro. rewrite -> H12 in H3.
-      apply int_cast_eq in H3.
+      injection H12. intro. rewrite H14 in H13.
+      apply int_cast_eq in H13.
       apply eq_intInteger.
       lia.
-      unfold new_base_val_binop in H3.
-      unfold base_val_binop in H3.
+      unfold new_base_val_binop in H13.
       destruct vb2.
-      discriminate.
-      discriminate. discriminate.
-      discriminate. discriminate.
-      discriminate. discriminate.
-      rewrite -> H12 in H11.
-      discriminate.
-      rewrite -> H12 in H11.
-      discriminate.
-      rewrite -> H3 in H11.
-      discriminate.
-      rewrite -> H3 in H11.
-      discriminate.
-      rewrite <- H3 in H11.
-      injection H6.
-      intro.
-      rewrite H11.
+      unfold base_val_binop in H13. all : try discriminate.
+      all : try rewrite -> H12 in H13. all : try discriminate.
+      all : try rewrite H12 in H0. all : try discriminate.
+      rewrite H0. 
       apply eq_intInteger.
       lia.
-    + rewrite H9 in H6.
-      rewrite <- H6.
+      
+    + rewrite H9 in H5.
+      rewrite <- H5.
       constructor.
       assumption.
 
     + destruct H2. discriminate.
       constructor.
       rewrite <- H4 in H1.
-      injection H6.
+      injection H5.
       intro.
       lia.
       apply eq_integerInt.
-      injection H6.
+      injection H5.
       lia.
       discriminate.
-      rewrite <- H6.
+      rewrite <- H5.
       constructor.
       assumption.
-    + destruct H2.
-      injection H6.
-      intro.
-      destruct H2. injection H6. intro. rewrite <- H8 in H2.
-      destruct vb2.
-      injection H6.
-      intro.
-      rewrite <- H8 in H00.
-      unfold valt_compop_ok in H00.
-      contradiction.
-      rewrite <- H8 in H00.
-      unfold valt_compop_ok in H00.
-      contradiction.
-      constructor.
-      apply int_cast_eq in H2.
-      lia.
-      rewrite <- H8 in H00.
       
-      unfold valt_compop_ok in H00.
-      contradiction.
-      rewrite <- H8 in H00.
-      unfold valt_compop_ok in H00.
-      contradiction.
-      discriminate.
-      rewrite H2 in H6. discriminate.
-      rewrite H2 in H6. discriminate.
-      rewrite H8 in H6. discriminate.
-      rewrite H8 in H6. discriminate. rewrite H2 in H6.
-      injection H6. intro. rewrite <- H6.
+    + destruct H2.
+      destruct H2. injection H5. intro. rewrite <- H8 in H7.
+      destruct vb2.
+      all : try rewrite <- H8 in H2.
+      all : try unfold base_val_binop_ok in H2.
+      all : try contradiction.
       constructor.
+      apply int_cast_eq in H7.
       lia.
-      discriminate.
-      discriminate.
+      all : try discriminate.
+      all : try rewrite H2 in H5. all : try discriminate.
+      all : try rewrite H7 in H5. all : try discriminate.
+      rewrite <- H5.
       constructor.
-      rewrite <- H5 in H1.
+      assumption.
+      rewrite <- H4 in H1.
       inversion H1.
-      lia.
-      rewrite <- H6.
       constructor.
       lia.
-    + destruct H2. discriminate. injection H6. intro. constructor. lia.
-      injection H6. intro. rewrite H7 in H3. rewrite H2 in H3. constructor. constructor.      
-      unfold new_base_val_binop. apply (int_cast_eq t t0 en x y0). assumption.
-      discriminate. rewrite <- H6. constructor. assumption.
+      rewrite <- H5.
+      constructor. assumption.
+     
+    + destruct H2. discriminate. injection H5. intro. constructor. lia.
+      injection H5. intro.  constructor. constructor. unfold base_val_binop_ok.
+      unfold int_binop_ok. exact I. 
+      unfold new_base_val_binop. apply (int_cast_eq t t0 en x y0). lia.
+      discriminate. rewrite <- H5. constructor. assumption.
     + assumption.
   Qed.
+
   
 End operations_definitions2.
+
